{
 "cells": [
  {
   "cell_type": "markdown",
   "id": "d1553b3e",
   "metadata": {},
   "source": [
    "### F-statistic ###"
   ]
  },
  {
   "cell_type": "markdown",
   "id": "e60f949e",
   "metadata": {},
   "source": [
    "In order to make **joint** hypothesis testing for the estimators $b_j$, define the null hypothesis:\n",
    "\n",
    "$$H_0 : R \\beta = r$$\n",
    "\n",
    "$$H_0 : R \\beta - r= 0$$\n",
    "\n",
    "Where $R_{g \\times k }$ is a matrix of $g$ number of restrictions imposed on the $k$ parameters, and $r_{g \\times 1}$ is a vector of values for these constraints (usually zero). \n",
    "\n",
    "For example, if $k = 3$, $g=2$, $r=0$ and $R$ is:\n",
    "\n",
    "$$R = \\begin{bmatrix}\n",
    "1 & 0 & 0 \\\\\n",
    "0 & 1 & 0 \\\\\n",
    "\\end{bmatrix}$$\n",
    "\n",
    "The null hypothesis is\n",
    "\n",
    "$$\n",
    "H_0 : \\begin{bmatrix}\n",
    "\\beta_1 \\\\\n",
    "\\beta_2 \\\\\n",
    "\\end{bmatrix}\n",
    "=\n",
    "\\begin{bmatrix}\n",
    "0 \\\\\n",
    "0 \\\\\n",
    "\\end{bmatrix}\n",
    "$$\n",
    "\n",
    "Remember: The $R$ and $r$ matrices do not need to be zeros and ones, you can make any linear combination to test. This could be testing whether $\\beta_1 = \\beta_2 + 1$, or $4\\beta_5 = \\beta_1 + 3\\beta_3 - 2$, etc.\n",
    "\n",
    "To test $ R \\beta - r= 0$ , we need to find a pivotal quantity. Recall that under assumptions 1-7, the distribution of $b$ is\n",
    "\n",
    "$$b \\sim N_k(\\beta, \\sigma^2(X^TX)^{-1})$$\n",
    "\n",
    "$$Rb \\sim N_g(R\\beta, \\sigma^2R(X^TX)^{-1}R^T)$$\n",
    "\n",
    "$$Rb - r \\sim N_g(R\\beta - r, \\sigma^2R(X^TX)^{-1}R^T)$$\n",
    "\n",
    "Under $H_0$, $R\\beta - r = 0$\n",
    "\n",
    "$$Rb - r \\sim N_g(0, \\sigma^2R(X^TX)^{-1}R^T)$$\n",
    "\n",
    "$$\\frac{Rb - r}{\\sigma} \\sim N_g(0, R(X^TX)^{-1}R^T)$$\n",
    "\n",
    "Rename $R(X^TX)^{-1}R^T = C_{g\\times g}$. If this matrix is positive definite and symmetric, it can be decomposed in $C = C^{\\frac{1}{2}}C^{\\frac{1}{2}}$\n",
    "\n",
    "$$\\frac{Rb - r}{\\sigma} \\sim N_g(0, C^{\\frac{1}{2}}C^{\\frac{1}{2}})$$\n",
    "\n",
    "$$C^{-\\frac{1}{2}}\\frac{Rb - r}{\\sigma} \\sim N_g(0, I_g)$$\n",
    "\n",
    "We would perform our tests with this using the $N_g(0,I_g)$ distribution, but notice that this is not yet a pivotal quantity, because there is an unknown $\\sigma$ parameter. We could adjust this using the Chi distribution and constructing $T$ random variables. However, this is not possible given that the distribution derived earlier estimates $\\sigma^2$, not $\\sigma$. We solve this constructing a Chi squared distribution from our $N_g(0, I_g)$\n",
    "\n",
    "$$C^{-\\frac{1}{2}}\\frac{Rb - r}{\\sigma} \\sim N_g(0, I_g) \\quad \\text{, then $\\Bigg[C^{-\\frac{1}{2}}\\frac{Rb - r}{\\sigma}\\Bigg]^TC^{-\\frac{1}{2}}\\frac{Rb - r}{\\sigma} \\sim \\chi^2(g)$}$$\n",
    "\n",
    "\n",
    "$$\\frac{(Rb - r)^TC^{-1}(Rb - r)}{\\sigma^2} \\sim \\chi^2(g)$$\n",
    "\n",
    "If $\\sigma$ were a know parameter, we would just use a Chi squared for the test. However, it isn't, so to find the pivotal quantity we will divide two Chi squared random variables, which will result in an $F$ random variable.\n",
    "\n",
    "For $V_1 \\sim \\chi^2(k_1)$ and $V_2 \\sim \\chi^2(k_2)$ Chi squared random variables:\n",
    "\n",
    "$$ F(k_1,k_2) = \\frac{V_1/k_1}{V_2/k_2} \\quad \\text{, an $F$ distribution with $k_1, k_2$ degrees of freedom} $$\n",
    "\n",
    "We will use $\\frac{e^Te}{\\sigma^2}$ , which we know from previous results that follows a $ \\chi^2(n-k)$ distribution. Then\n",
    "\n",
    "\n",
    "$$\\frac{V_1/k_1}{V_2/k_2} = \\frac{(Rb - r)^TC^{-1}(Rb - r)}{\\sigma^2}\\frac{1}{g}\\Bigg[\\frac{e^Te}{\\sigma^2}\\frac{1}{n-k}\\Bigg]^{-1} = \\frac{(Rb - r)^TC^{-1}(Rb - r)/g}{e^Te/(n-k)} \\sim F(g,n-k)$$\n",
    "\n",
    "Where $C = R(X^TX)^{-1}R^T$\n",
    "\n"
   ]
  },
  {
   "cell_type": "markdown",
   "id": "c764bec0",
   "metadata": {},
   "source": [
    "### Restricted regression ###"
   ]
  },
  {
   "cell_type": "markdown",
   "id": "a29b3bdb",
   "metadata": {},
   "source": [
    "To find the $b_R$ estimators that minimize the sum of squared residuals, subject to having a constraint of the form  $Rb_R = r$:\n",
    "\n",
    "\\begin{equation*}\n",
    "\\begin{aligned}\n",
    "& \\underset{b_R}{\\text{minimize}}\n",
    "& & S(b_R) = (y-Xb_R)^T(y-Xb_R) \\\\\n",
    "& \\text{subject to}\n",
    "& & Rb_R - r = g(b_R) = 0.\n",
    "\\end{aligned}\n",
    "\\end{equation*}\n",
    "\n",
    "The Karush-Kuhn-Tucker conditions are:\n",
    "\n",
    "$$\\nabla S(b_R) = \\nabla g(b_R) \\lambda $$\n",
    "\n",
    "$$g(b_R) =0  $$\n",
    "\n",
    "$$ X^T(y-Xb_R) = R^T \\lambda $$\n",
    "\n",
    "$$ (X^TX)b_R = X^Ty - R^T\\lambda$$\n",
    "\n",
    "$$ b_R = (X^TX)^{-1}X^Ty - (X^TX)^{-1}R^T\\lambda$$\n",
    "\n",
    "Where $b = (X^TX)^{-1}X^Ty$ is the estimator from the non restricted model\n",
    "\n",
    "$$ b_R = b - (X^TX)^{-1}R^T\\lambda$$\n",
    "\n",
    "Premultiplying bt $R$ and substracting $r$\n",
    "\n",
    "$$ Rb_R - r = Rb - R(X^TX)^{-1}R^T\\lambda - r $$\n",
    "\n",
    "$$R(X^TX)^{-1}R^T\\lambda = Rb - r $$\n",
    "\n",
    "$$\\lambda = (R(X^TX)^{-1}R^T)^{-1}(Rb - r) $$\n",
    "\n",
    "Replacing:\n",
    "\n",
    "$$ b_R = b - (X^TX)^{-1}R^T(R(X^TX)^{-1}R^T)^{-1}(Rb - r)$$\n",
    "\n",
    "Using $y = Xb + e$ and $y = Xb_R + e_R$ \n",
    "\n",
    "$$ Xb_R = Xb - X(X^TX)^{-1}R^T(R(X^TX)^{-1}R^T)^{-1}(Rb - r)$$\n",
    "\n",
    "$$ y - e_R = y - e - X(X^TX)^{-1}R^T(R(X^TX)^{-1}R^T)^{-1}(Rb - r)$$\n",
    "\n",
    "$$ e_R = e + X(X^TX)^{-1}R^T(R(X^TX)^{-1}R^T)^{-1}(Rb - r)$$\n",
    "\n",
    "$$ e_R^T = e^T + (Rb - r)^T(R(X^TX)^{-1}R^T)^{-1}R(X^TX)^{-1}X^T $$\n",
    "\n",
    "Using the fact that $X^Te = 0$, and renaming $C = R(X^TX)^{-1}R^T$\n",
    "\n",
    "$$e_R^Te_R = e^Te + (Rb - r)^T(R(X^TX)^{-1}R^T)^{-1}R(X^TX)^{-1}X^TX(X^TX)^{-1}R^T(R(X^TX)^{-1}R^T)^{-1}(Rb - r)   $$\n",
    "\n",
    "(The following also counts as a proof that when a model is restricted, its SSR increases)\n",
    "\n",
    "$$e_R^Te_R = e^Te + (Rb - r)^TC^{-1}CC^{-1}(Rb - r)   $$\n",
    "\n",
    "$$e_R^Te_R - e^Te = (Rb - r)^TC^{-1}(Rb - r)   $$\n",
    "\n",
    "Finally, we can replace this result in the $F$ statistic:\n",
    "\n",
    "$$F = \\frac{(Rb - r)^TC^{-1}(Rb - r)/g}{e^Te/(n-k)} = \\frac{(e_R^Te_R - e^Te)/g}{e^Te/(n-k)}    \\sim F(g,n-k)$$\n",
    "\n",
    "In terms of $SSR$\n",
    "\n",
    "$$F = \\frac{(SSR_R - SSR)/g}{SSR/(n-k)}   $$\n",
    "\n",
    "So we can test the **joint** hypothesis using as input for the $F$ statistic the $SSR$ of both specifications. "
   ]
  },
  {
   "cell_type": "code",
   "execution_count": null,
   "id": "bbb3718e",
   "metadata": {},
   "outputs": [],
   "source": []
  }
 ],
 "metadata": {
  "kernelspec": {
   "display_name": "Python 3 (ipykernel)",
   "language": "python",
   "name": "python3"
  },
  "language_info": {
   "codemirror_mode": {
    "name": "ipython",
    "version": 3
   },
   "file_extension": ".py",
   "mimetype": "text/x-python",
   "name": "python",
   "nbconvert_exporter": "python",
   "pygments_lexer": "ipython3",
   "version": "3.11.5"
  }
 },
 "nbformat": 4,
 "nbformat_minor": 5
}
